\begin{itemize}
    \item $k *C^k_n=n*C^{k-1}_{n-1}$ ；
    \item $C_k^n*C_m^k=C_m^n*C_{m-n}^{m-k}$ ；
    \item $C_n^k+C_n^{k+1}=C_{n+1}^{k+1}$ ；
    \item $\sum_{i=0}^n C_n^i=2^n$ ；
    \item $\sum_{k=0}^n(-1)^k*C_n^k=0$ 。
    \item 二项式反演：$\left\{\begin{matrix} \displaystyle f_n=\sum_{i=0}^n{n\choose i}g_i\Leftrightarrow g_n=\sum_{i=0}^n(-1)^{n-i}{n\choose i}f_i \\
                  \displaystyle f_k=\sum_{i=k}^n{i\choose k}g_i\Leftrightarrow g_k=\sum_{i=k}^n(-1)^{i-k}{i\choose k}f_i\end{matrix}\right. $ ；
    \item $\displaystyle \sum_{i=1}^{n}i{n\choose i}=n * 2^{n-1}$ ；
    \item $\displaystyle \sum_{i=1}^{n}i^2{n\choose i}=n*(n+1)*2^{n-2}$ ；
    \item $\displaystyle \sum_{i=1}^{n}\dfrac{1}{i}{n\choose i}=\sum_{i=1}^{n}\dfrac{1}{i}$ ；
    \item $\displaystyle \sum_{i=0}^{n}{n\choose i}^2={2n\choose n}$ ；
    \item 拉格朗日恒等式：$\displaystyle \sum_{i=1}^{n}\sum_{j=i+1}^{n}(a_ib_j-a_jb_i)^2=(\sum_{i=1}^{n}a_i)^2(\sum_{i=1}^{n}b_i)^2-(\sum_{i=1}^{n}a_ib_i)^2$ 。
\end{itemize}